Back to standard coinduction for now
Proof automation appears to be slightly less straightforward in Paco,
let us see if standard coinduction is more forthcoming.

The proofs as they stand now are compatible with both standard
coinduction and parameterized coinduction. Summary of changes:

 - Inductive generators are transformed into standard coinductive
   definitions, where coinductive calls replace the parametric
   relation (and parameters that were implicit in the latter are added
   to the former). All entries in hint databases are preserved.

 - In proofs, Paco tactics ([pcofix], [pinversion], etc.) are replaced
   by their standard equivalents. Unfolding tactics ([pfold],
   [punfold]) and the selection of left of right disjuncts on Paco
   definitions are removed.

 - Doing so results in proofs that are essentially valid for both
   standard and parameterized coinduction. The only exceptions are
   occasional sub-goals that can be discharged from the context in
   standard coinduction and require a little extra unfolding work in
   Paco, or occasionally an application of monotonicity.

"Non-trivial" (yet quite trivial, actually) differences are left in
comments for reference.

ObsTrace.v
@@ -18,25 +18,25 @@ Ltac app_frobber :=
 
 (********************** ObsTrace Equivalence *************************)
 
-Inductive ObsTraceEq_gen R : TraceOf Observation -> TraceOf Observation -> Prop :=
+CoInductive ObsTraceEq(*_gen R*) : TraceOf Observation -> TraceOf Observation -> Prop :=
 | ObsEqTau1 : forall OO OO'
-                     (HR : R OO OO' : Prop),
-    ObsTraceEq_gen R (notfinished Tau OO) OO'
+                     (HR : (*R*)ObsTraceEq OO OO' : Prop),
+    ObsTraceEq(*_gen R*) (notfinished Tau OO) OO'
 | ObsEqTau2 : forall OO OO'
-                     (HR : R OO OO' : Prop),
-    ObsTraceEq_gen R OO (notfinished Tau OO')
+                     (HR : (*R*)ObsTraceEq OO OO' : Prop),
+    ObsTraceEq(*_gen R*) OO (notfinished Tau OO')
 | ObsEqNow : forall w OO OO'
-                     (HR : R OO OO' : Prop),
-    ObsTraceEq_gen R (notfinished (Out w) OO) (notfinished (Out w) OO')
+                     (HR : (*R*)ObsTraceEq OO OO' : Prop),
+    ObsTraceEq(*_gen R*) (notfinished (Out w) OO) (notfinished (Out w) OO')
 | ObsEqFinishedOut : forall w,
-    ObsTraceEq_gen R (finished (Out w)) (finished (Out w))
+    ObsTraceEq(*_gen R*) (finished (Out w)) (finished (Out w))
 | ObsEqFinishedTau :
-    ObsTraceEq_gen R (finished Tau) (finished Tau)
+    ObsTraceEq(*_gen R*) (finished Tau) (finished Tau)
 (* The last thing we need is a way of handling *all-tau* traces.
    There are a couple of ways of doing that, not sure what will
    play better in proofs. *)
 | ObsEqAllTau : forall OO,
-     ObsTraceEq_gen R OO OO.
+     ObsTraceEq(*_gen R*) OO OO.
 (* APT: Establishing equality between traces seems hard, and this overlaps
 the previous two cases.  Maybe try:
    ForallTrace (fun o => o = Tau) OO ->
@@ -46,13 +46,13 @@ the previous two cases.  Maybe try:
 LEO: That was the other thing I had in mind. I'll see what makes proofs easier.
 (Note that this proposal overlaps with the first two cases, as well as the last one.)
  *)
-Hint Constructors ObsTraceEq_gen : core.
+Hint Constructors ObsTraceEq(*_gen*) : core.
 
-Definition ObsTraceEq (OO OO' : TraceOf Observation) :=
-  paco2 ObsTraceEq_gen bot2 OO OO'.
-Hint Unfold ObsTraceEq : core.
-Lemma ObsTraceEq_mon : monotone2 ObsTraceEq_gen. Proof. pmonauto. Qed.
-Hint Resolve ObsTraceEq_mon : paco.
+(* Definition ObsTraceEq (OO OO' : TraceOf Observation) := *)
+(*   paco2 ObsTraceEq_gen bot2 OO OO'. *)
+(* Hint Unfold ObsTraceEq : core. *)
+(* Lemma ObsTraceEq_mon : monotone2 ObsTraceEq_gen. Proof. pmonauto. Qed. *)
+(* Hint Resolve ObsTraceEq_mon : paco. *)
 
 Notation "OO' ~=_O OO" := (ObsTraceEq OO' OO) (at level 80).
 
@@ -60,42 +60,45 @@ Lemma ObsTraceEq_sym :
   forall O O',
     ObsTraceEq O O' -> ObsTraceEq O' O.
 Proof.
-  pcofix COFIX.
-  intros O O' H; pfold.
+  cofix COFIX.
+  intros O O' H(*; pfold*).
   inv H;
-    try (constructor; (right; apply COFIX; auto) || (left; auto)).
+    try (constructor; ((*right;*) apply COFIX; auto) || ((*left;*) auto)).
+    (* Or, simplified, [constructor; auto]. *)
 Qed.
 
 Lemma ObsTraceEqRemoveTau1 :
   forall T T', ObsTraceEq (notfinished Tau T) T' -> ObsTraceEq T T'.
 Proof.
-  pcofix COFIX.
-  intros T T' Eq; pfold.
+  cofix COFIX.
+  intros T T' Eq(*; pfold*).
   inv Eq.
   + (* RB: This goal is slightly more involved than it was before. *)
-    apply paco2_unfold.
-    * apply ObsTraceEq_mon.
-    * apply paco2_mon_bot with ObsTraceEq_gen; auto.
+    (* apply paco2_unfold. *)
+    (* * apply ObsTraceEq_mon. *)
+    (* * apply paco2_mon_bot with ObsTraceEq_gen; auto. *)
+    assumption.
   + eapply ObsEqTau2.
-    right. eapply COFIX; auto.
+    (*right.*) eapply COFIX; auto.
   + eapply ObsEqTau2.
-    left. pfold. eapply ObsEqAllTau.
+    (*left. pfold.*) eapply ObsEqAllTau.
 Qed.
 
 Lemma ObsTraceEqRemoveTau2 :
   forall T T', ObsTraceEq T (notfinished Tau T') -> ObsTraceEq T T'.
 Proof.
-  pcofix COFIX.
-  intros T T' Eq; pfold.
+  cofix COFIX.
+  intros T T' Eq(*; pfold*).
   inv Eq.
   + eapply ObsEqTau1.
-    right. eapply COFIX.
+    (*right.*) eapply COFIX.
     auto.
   + (* RB: This goal is slightly more involved than it was before. *)
-    apply paco2_unfold.
-    * apply ObsTraceEq_mon.
-    * apply paco2_mon_bot with ObsTraceEq_gen; auto.
-  + eapply ObsEqTau1. left. pfold.
+    (* apply paco2_unfold. *)
+    (* * apply ObsTraceEq_mon. *)
+    (* * apply paco2_mon_bot with ObsTraceEq_gen; auto. *)
+    assumption.
+  + eapply ObsEqTau1. (*left. pfold.*)
     eapply ObsEqAllTau.
 Qed.
 
@@ -114,7 +117,7 @@ Proof.
   intros T' t' HL.
   induction HL; intros w Tw Eq.
   - exists 0. left. simpl.
-    pinversion Eq.
+    inversion Eq.
   - destruct a'.
     + inv Eq.
       * exists 0.
@@ -152,15 +155,15 @@ Proof.
     generalize dependent O2';
     generalize dependent Eq1.
     induction Last';
-      intros Eq1 O2' O2 Eq2;
-      pfold.
-    + pinversion Eq1; subst; simpl in *; clear Eq1; app_frobber.
+      intros Eq1 O2' O2 Eq2(*;
+      pfold*).
+    + inversion Eq1; subst; simpl in *; clear Eq1; app_frobber.
       * apply ObsEqNow; auto.
-      * apply ObsEqTau1. left. pfold. apply ObsEqTau2; auto.
+      * apply ObsEqTau1. (*left. pfold.*) apply ObsEqTau2; auto.
       * destruct a.
         -- apply ObsEqNow; auto.
-        -- apply ObsEqTau1. left. pfold. apply ObsEqTau2; auto.
-    + pinversion Eq1; subst; simpl in *; clear Eq1.
+        -- apply ObsEqTau1. (*left. pfold.*) apply ObsEqTau2; auto.
+    + inversion Eq1; subst; simpl in *; clear Eq1.
       specialize (IHLast' HR O2' O2 Eq2).
       app_frobber.
       eapply ObsEqTau2.
@@ -169,9 +172,9 @@ Proof.
     + destruct (EqOut_tauN O1' o1' Last' w T Eq1) as [n [HTau | [T' HTau]]].
       * rewrite HTau in *.
         clear HTau.
-        induction n; simpl in *; subst; app_frobber; pfold.
+        induction n; simpl in *; subst; app_frobber(*; pfold*).
         -- apply ObsEqNow.
-           pinversion Eq1.
+           inversion Eq1.
         -- apply ObsEqTau2.
            inversion Last'; subst; clear Last'.
            apply ObsTraceEqRemoveTau2 in Eq1.
@@ -179,15 +182,15 @@ Proof.
            auto.
       * rewrite HTau in *.
         clear HTau.
-        induction n; simpl in *; subst; app_frobber; pfold.
+        induction n; simpl in *; subst; app_frobber(*; pfold*).
         -- apply ObsEqNow.
-           pinversion Eq1; subst; clear Eq1.
+           inversion Eq1; subst; clear Eq1.
            (* RB: The following two subgoals become slightly different. *)
            ++ inversion Last'; subst; clear Last'.
-              left.
+              (*left.*)
               eapply IHLast; eauto.
            ++ inversion Last'; subst; clear Last'.
-              left.
+              (*left.*)
               eapply IHLast; eauto.
         -- inversion Last'; subst; clear Last'.
            specialize (IHn H3).
@@ -198,7 +201,7 @@ Proof.
     + apply ObsTraceEqRemoveTau1 in Eq1.
       app_frobber.
       (* RB: Ditto here, applying IH is now a bit more explicit. *)
-      pfold. apply ObsEqTau1. left.
+      (*pfold.*) apply ObsEqTau1. (*left.*)
       eapply IHLast; eauto.
 Qed.
 
@@ -210,31 +213,31 @@ Definition ObsTracePrefix (OO OO' : TraceOf Observation) : Prop :=
  *)
 
 (* The second is a prefix of the first, up to Tau *)
-Inductive ObsTracePrefix_gen R : TraceOf Observation -> TraceOf Observation -> Prop :=
+CoInductive ObsTracePrefix(*_gen R*) : TraceOf Observation -> TraceOf Observation -> Prop :=
 | ObsPreTau1 : forall OO OO'
-                      (HR : R OO OO' : Prop),
-    ObsTracePrefix_gen R (notfinished Tau OO) OO'
+                      (HR : (*R*)ObsTracePrefix OO OO' : Prop),
+    ObsTracePrefix(*_gen R*) (notfinished Tau OO) OO'
 | ObsPreTau2 : forall OO OO'
-                      (HR : R OO OO' : Prop),
-    ObsTracePrefix_gen R OO (notfinished Tau OO')
+                      (HR : (*R*)ObsTracePrefix OO OO' : Prop),
+    ObsTracePrefix(*_gen R*) OO (notfinished Tau OO')
 | ObsPreNow : forall w OO OO'
-                      (HR : R OO OO' : Prop),
-    ObsTracePrefix_gen R (notfinished (Out w) OO) (notfinished (Out w) OO')
+                      (HR : (*R*)ObsTracePrefix OO OO' : Prop),
+    ObsTracePrefix(*_gen R*) (notfinished (Out w) OO) (notfinished (Out w) OO')
 | ObsPreFinishedOut1 : forall w,
-    ObsTracePrefix_gen R (finished (Out w)) (finished (Out w))
+    ObsTracePrefix(*_gen R*) (finished (Out w)) (finished (Out w))
 | ObsPreFinishedOut2 : forall w OO,
-    ObsTracePrefix_gen R (notfinished (Out w) OO) (finished (Out w))
+    ObsTracePrefix(*_gen R*) (notfinished (Out w) OO) (finished (Out w))
 | ObsPreFinishedTau : forall OO,
-    ObsTracePrefix_gen R OO (finished Tau)
+    ObsTracePrefix(*_gen R*) OO (finished Tau)
 | ObsPreAllTau : forall OO,
-     ObsTracePrefix_gen R OO OO.
-Hint Constructors ObsTracePrefix_gen : core.
+     ObsTracePrefix(*_gen R*) OO OO.
+Hint Constructors ObsTracePrefix(*_gen*) : core.
 
-Definition ObsTracePrefix (OO OO' : TraceOf Observation) :=
-  paco2 ObsTracePrefix_gen bot2 OO OO'.
-Hint Unfold ObsTracePrefix : core.
-Lemma ObsTracePrefix_mon : monotone2 ObsTracePrefix_gen. Proof. pmonauto. Qed.
-Hint Resolve ObsTracePrefix_mon : paco.
+(* Definition ObsTracePrefix (OO OO' : TraceOf Observation) := *)
+(*   paco2 ObsTracePrefix_gen bot2 OO OO'. *)
+(* Hint Unfold ObsTracePrefix : core. *)
+(* Lemma ObsTracePrefix_mon : monotone2 ObsTracePrefix_gen. Proof. pmonauto. Qed. *)
+(* Hint Resolve ObsTracePrefix_mon : paco. *)
 
 Notation "OO' <=_O OO" := (ObsTracePrefix OO OO') (at level 80).
 
@@ -253,28 +256,28 @@ Proof.
     generalize dependent O2';
     generalize dependent Eq.
     induction Last';
-      intros Eq O2' O2 Pref; pfold.
-    + pinversion Eq; subst; simpl in *; clear Eq; app_frobber.
+      intros Eq O2' O2 Pref(*; pfold*).
+    + inversion Eq; subst; simpl in *; clear Eq; app_frobber.
       (* Hint constructors doesn't work for this? *)
       * apply ObsPreNow; auto.
-      * apply ObsPreTau1. left. pfold. apply ObsPreTau2; auto.
+      * apply ObsPreTau1. (*left. pfold.*) apply ObsPreTau2; auto.
       * destruct a.
         -- apply ObsPreNow; auto.
-        -- apply ObsPreTau1. left. pfold. apply ObsPreTau2; auto.
-    + pinversion Eq; subst; simpl in *; clear Eq.
+        -- apply ObsPreTau1. (*left. pfold.*) apply ObsPreTau2; auto.
+    + inversion Eq; subst; simpl in *; clear Eq.
       specialize (IHLast' HR O2' O2 Pref).
       app_frobber.
       eapply ObsPreTau2.
       auto.
   (* Try by inversion. *)
   - destruct a'.
-    + destruct (EqOut_tauN O1' o1' Last' w T Eq) as [n [HTau | [T' HTau]]];
-        pfold.
+    + destruct (EqOut_tauN O1' o1' Last' w T Eq) as [n [HTau | [T' HTau]]](*;
+        pfold*).
       * rewrite HTau in *.
         clear HTau.
         induction n; simpl in *; subst; app_frobber.
         -- apply ObsPreNow.
-           pinversion Eq. (* This makes me feel strange *)
+           inversion Eq. (* This makes me feel strange *)
         -- apply ObsPreTau2.
            inversion Last'; subst; clear Last'.
            apply ObsTraceEqRemoveTau2 in Eq.
@@ -284,13 +287,13 @@ Proof.
         clear HTau.
         induction n; simpl in *; subst; app_frobber.
         -- apply ObsPreNow.
-           pinversion Eq; subst; clear Eq.
+           inversion Eq; subst; clear Eq.
            (* RB: The following two subgoals become slightly different. *)
            ++ inversion Last'; subst; clear Last'.
-              left.
+              (*left.*)
               eapply IHLast; eauto.
            ++ inversion Last'; subst; clear Last'.
-              left.
+              (*left.*)
               eapply IHLast; eauto.
         -- inversion Last'; subst; clear Last'.
            specialize (IHn H3).
@@ -300,21 +303,21 @@ Proof.
            auto.
     + apply ObsTraceEqRemoveTau1 in Eq.
       app_frobber.
-      pfold. apply ObsPreTau1. left.
+      (*pfold.*) apply ObsPreTau1. (*left.*)
       (* RB: Ditto here, applying IH is now a bit more explicit. *)
       eapply IHLast; eauto.
 Qed.
 
 Lemma ObsTracePrefix_refl : forall OO, ObsTracePrefix OO OO.
 Proof.
-  pcofix CH.
-  intros [o | o OO]; pfold.
+  cofix CH.
+  intros [o | o OO](*; pfold*).
   - destruct o as [w |].
     + now apply ObsPreFinishedOut1.
     + now apply ObsPreFinishedTau.
   - destruct o as [w |].
     + apply ObsPreNow. now auto.
-    + apply ObsPreTau1. left. pfold. apply ObsPreTau2. now auto.
+    + apply ObsPreTau1. (*left. pfold.*) apply ObsPreTau2. now auto.
 Qed.
 
 
@@ -326,11 +329,11 @@ Lemma TraceEqImpliesObsTraceEq :
     O ~= O' ->
     ObsTraceEq O O'.
 Proof.
-  pcofix COFIX. intros O O' H; pfold. inv H.
+  cofix COFIX. intros O O' H(*; pfold*). inv H.
   - constructor.
   - destruct a.
     + constructor. auto.
-    + constructor. left. pfold. constructor. auto.
+    + constructor. (*left. pfold.*) constructor. auto.
 Qed.
 
 Lemma ObsTraceEqImpliesPrefix :
@@ -338,23 +341,24 @@ Lemma ObsTraceEqImpliesPrefix :
     ObsTraceEq O O' ->
     O <=_O O'.
 Proof.
-  pcofix COFIX. intros O O' H. pfold.
-  inv H; constructor; right; apply COFIX; auto.
+  cofix COFIX. intros O O' H. (*pfold.*)
+  inv H; constructor; (*right;*) apply COFIX; auto.
 Qed.
 
 Lemma ObsTracePrefRemoveTau1 :
   forall T T', (notfinished Tau T) <=_O T' -> T <=_O T'.
 Proof.
-  pcofix COFIX.
-  intros T T' Pref; pfold.
+  cofix COFIX.
+  intros T T' Pref(*; pfold*).
   inv Pref.
-  + constructor. right. apply COFIX. auto.
+  + constructor. (*right.*) apply COFIX. auto.
   + (* RB: Some base cases like this need a little more work than before. *)
-    apply paco2_unfold.
-    * auto with paco.
-    * eapply paco2_mon_bot; eauto with paco.
-  + constructor. left.
-    eapply paco2_mon_bot with ObsTracePrefix_gen; [| auto].
+    (* apply paco2_unfold. *)
+    (* * auto with paco. *)
+    (* * eapply paco2_mon_bot; eauto with paco. *)
+    assumption.
+  + constructor. (*left.
+    eapply paco2_mon_bot with ObsTracePrefix_gen; [| auto].*)
     apply ObsTracePrefix_refl.
 Qed.
 
@@ -364,22 +368,24 @@ Lemma ObsPrefOverEq :
     O1 <=_O O2 ->
     O1' <=_O O2.
 Proof.
-  pcofix COFIX. intros O1 O1' O2 H H0; pfold. inv H.
-  - apply paco2_unfold.
-    + auto with paco.
-    + eapply paco2_mon_bot; eauto with paco.
+  cofix COFIX. intros O1 O1' O2 H H0(*; pfold*). inv H.
+  - assumption.
+    (* apply paco2_unfold. *)
+    (* + auto with paco. *)
+    (* + eapply paco2_mon_bot; eauto with paco. *)
   - destruct a.
     + inv H0.
-      * constructor. right.
+      * constructor. (*right.*)
         apply (COFIX (notfinished (Out w) T1) (notfinished (Out w) T2) OO).
-        -- pfold. constructor. auto.
+        -- (*pfold.*) constructor. auto.
         -- auto.
-      * constructor. right. apply (COFIX T1 T2 OO); auto.
-      * constructor. left.
-        apply paco2_mon_bot with ObsTracePrefix_gen; [| auto].
+      * constructor. (*right.*) apply (COFIX T1 T2 OO); auto.
+      * constructor.
+        (* left. *)
+        (* apply paco2_mon_bot with ObsTracePrefix_gen; [| auto]. *)
         apply ObsTraceEqImpliesPrefix. apply TraceEqImpliesObsTraceEq in H1.
         apply ObsTraceEq_sym. auto.
-    + constructor. right. apply (COFIX T1 T2 O2); auto. apply ObsTracePrefRemoveTau1. auto.
+    + constructor. (*right.*) apply (COFIX T1 T2 O2); auto. apply ObsTracePrefRemoveTau1. auto.
 Qed.
 
 Lemma ObsEqOverEq :
@@ -388,19 +394,21 @@ Lemma ObsEqOverEq :
     ObsTraceEq O1 O2 ->
     ObsTraceEq O1' O2.
 Proof.
-  pcofix COFIX. intros O1 O1' O2 H H0; pfold. inv H.
-  - apply paco2_unfold.
-    * auto with paco.
-    * eapply paco2_mon_bot; eauto with paco.
+  cofix COFIX. intros O1 O1' O2 H H0(*; pfold*). inv H.
+  - assumption.
+    (* apply paco2_unfold. *)
+    (* * auto with paco. *)
+    (* * eapply paco2_mon_bot; eauto with paco. *)
   - destruct a.
     + inv H0.
-      * constructor. right.
+      * constructor. (*right.*)
         apply (COFIX (notfinished (Out w) T1) (notfinished (Out w) T2) OO').
-        -- pfold. constructor. auto.
+        -- (*pfold.*) constructor. auto.
         -- auto.
-      * constructor. right. apply (COFIX T1 T2 OO'); auto.
-      * constructor. left.
-        apply paco2_mon_bot with ObsTraceEq_gen; [| auto].
+      * constructor. (*right.*) apply (COFIX T1 T2 OO'); auto.
+      * constructor.
+        (* left. *)
+        (* apply paco2_mon_bot with ObsTraceEq_gen; [| auto]. *)
         apply ObsTraceEq_sym. apply TraceEqImpliesObsTraceEq. auto.
-    + constructor. right. apply (COFIX T1 T2 O2); auto. apply ObsTraceEqRemoveTau1. auto.
+    + constructor. (*right.*) apply (COFIX T1 T2 O2); auto. apply ObsTraceEqRemoveTau1. auto.
 Qed.
